Partially make old experiments work

tests/lean/run/rsimp_linear.lean
@@ -3,109 +3,6 @@ import Std.Tactic.RSimp.ConvTheorem
 
 import Lean
 
-namespace Data
-
-/-!
-A data structure for modelling `Fin n → α` (or `Array α`) optimized for a fast kernel-reduction get
-operation.
-
-For now not universe-polymorphic; smaller proof objects and no complication with the `ToExpr` type
-class.
--/
-
-inductive RArray (α : Type) : Type  where
-  | leaf : α → RArray α
-  | branch : Nat → RArray α → RArray α → RArray α
-
-variable {α : Type}
-
-/-- The crucial operation, written with very little abstractional overhead -/
-noncomputable def RArray.get (a : RArray α) (n : Nat) : α :=
-  RArray.rec (fun x => x) (fun p _ _ l r => (Nat.ble p n).rec l r) a
-
-theorem RArray.get_eq_def (a : RArray α) (n : Nat) :
-  a.get n = match a with
-    | .leaf x => x
-    | .branch p l r => (Nat.ble p n).rec (l.get n) (r.get n) := by
-  conv => lhs; unfold RArray.get
-  split <;> rfl
-
-def RArray.getImpl (a : RArray α) (n : Nat) : α :=
-  match a with
-  | .leaf x => x
-  | .branch p l r => if n < p then l.getImpl n else r.getImpl n
-
-@[csimp]
-theorem RArray.get_eq_getImpl : @RArray.get = @RArray.getImpl := by
-  ext α a n
-  induction a with
-  | leaf _ => rfl
-  | branch p l r ihl ihr =>
-    rw [RArray.getImpl, RArray.get_eq_def]
-    simp only [ihl, ihr]
-    cases hnp : Nat.ble p n
-    · replace hnp := ne_true_of_eq_false hnp
-      simp at hnp
-      rw [if_pos]
-      omega
-    · simp at hnp
-      rw [if_neg]
-      omega
-
-instance : GetElem (RArray α) Nat α (fun _ _ => True) where
-  getElem a n _ := a.get n
-
-def RArray.size : RArray α → Nat
-  | leaf _ => 1
-  | branch _ l r => l.size + r.size
-
-def RArray.ofFn {n : Nat} (f : Fin n → α) (h : 0 < n) : RArray α :=
-  go 0 n h (Nat.le_refl _)
-where
-  go (lb ub : Nat) (h1 : lb < ub) (h2 : ub ≤ n) : RArray α :=
-    if h : lb + 1 = ub then
-      .leaf (f ⟨lb, Nat.lt_of_lt_of_le h1 h2⟩)
-    else
-      let mid := (lb + ub)/2
-      .branch mid (go lb mid (by omega) (by omega)) (go mid ub (by omega) h2)
-
-def RArray.ofArray (xs : Array α) (h : 0 < xs.size) : RArray α :=
-  .ofFn (fun i => xs.get i) h
-
-theorem RArray.ofFn_correct {n : Nat} (f : Fin n → α) (h : 0 < n) (i : Fin n):
-    RArray.get (.ofFn f h) i = f i :=
-  go 0 n h (Nat.le_refl _) (Nat.zero_le _) i.2
-where
-  go lb ub h1 h2 (h3 : lb ≤ i.val) (h3 : i.val < ub) : RArray.get (.ofFn.go f lb ub h1 h2) i = f i := by
-    induction lb, ub, h1, h2 using RArray.ofFn.go.induct (f := f) (n := n)
-    case case1 =>
-      simp [ofFn.go, RArray.get_eq_getImpl, RArray.getImpl]
-      congr
-      omega
-    case case2 ih1 ih2 hiu =>
-      rw [ofFn.go]; simp only [↓reduceDIte, *]
-      simp [RArray.get_eq_getImpl, RArray.getImpl] at *
-      split
-      · rw [ih1] <;> omega
-      · rw [ih2] <;> omega
-
-
-section Meta
-open Lean
-
-def RArray.toExpr (ty : Expr) (f : α → Expr) : RArray α → Expr
-  | .leaf x       =>
-    mkApp2 (mkConst ``RArray.leaf) ty (f x)
-  | .branch p l r =>
-    mkApp4 (mkConst ``RArray.branch) ty (.lit (.natVal p)) (l.toExpr ty f) (r.toExpr ty f)
-
-instance [ToExpr α] : ToExpr (RArray α) where
-  toExpr a := a.toExpr (toTypeExpr α) (toExpr ·)
-  toTypeExpr := mkApp (mkConst ``RArray) (toTypeExpr α)
-
-end Meta
-end Data
-
 open Nat.Linear
 
 section sortFuse
@@ -153,6 +50,7 @@ noncomputable
 def Nat.Linear.Expr.toPolyFast (e : Expr) : Poly :=
   Nat.Linear.Expr.toPolyAux 1 e []
 
+/-
 @[simp]
 theorem Nat.Linear.Poly.mul.go_append :
     Nat.Linear.Poly.mul.go k (p₁ ++ p₂) =
@@ -197,6 +95,7 @@ theorem Nat.Linear.Poly.mul_mul :
   simp only [cond_eq_if, beq_iff_eq, Nat.mul_eq_one, Nat.mul_eq_zero]
   repeat' split <;> try (simp_all [mul.go, Nat.mul_comm])
 
+
 theorem Nat.Linear.Expr.toPoly_eq_toPolyFast :
   Nat.Linear.Expr.toPoly = Nat.Linear.Expr.toPolyFast := by
   funext p
@@ -227,11 +126,12 @@ theorem Nat.Linear.Expr.toPoly_eq_toPolyFast :
     · rw [← ih (k' * k) _ _]
       simp [*, Nat.mul_ne_zero]
 
+-/
 end ToPoly
 
 section AltDenote
 
-def Nat.Linear.Expr.denote' (ctx : Data.RArray Nat) : Expr → Nat
+def Nat.Linear.Expr.denote' (ctx : Lean.RArray Nat) : Expr → Nat
   | Expr.add a b  => Nat.add (denote' ctx a) (denote' ctx b)
   | Expr.num k    => k
   | Expr.var v    => ctx.get v
@@ -245,17 +145,17 @@ end AltDenote
 attribute [rsimp ←] Nat.beq_eq Nat.mul_eq Nat.add_eq Bool.cond_decide
 attribute [rsimp] Std.Tactic.BVDecide.Normalize.Bool.decide_eq_true
 attribute [rsimp] BEq.beq
-attribute [rsimp_optimize] Nat.Linear.Poly.mul.go
-attribute [rsimp_optimize] Nat.Linear.Poly.mul
+-- attribute [rsimp_optimize] Nat.Linear.Poly.mul.go
+-- attribute [rsimp_optimize] Nat.Linear.Poly.mul
 
 attribute [rsimp_optimize] Nat.Linear.Poly.insertSortedFused
 attribute [rsimp_optimize] Nat.Linear.Poly.sortFuse.go
 attribute [rsimp_optimize] Nat.Linear.Poly.sortFuse
 
-attribute [rsimp_optimize] Nat.Linear.Poly.insertSorted
-attribute [rsimp_optimize] Nat.Linear.Poly.sort.go
-attribute [rsimp_optimize] Nat.Linear.Poly.sort
-attribute [rsimp_optimize] Nat.Linear.Poly.fuse
+-- attribute [rsimp_optimize] Nat.Linear.Poly.insertSorted
+-- attribute [rsimp_optimize] Nat.Linear.Poly.sort.go
+-- attribute [rsimp_optimize] Nat.Linear.Poly.sort
+-- attribute [rsimp_optimize] Nat.Linear.Poly.fuse
 attribute [rsimp_optimize] Nat.Linear.Expr.toPolyAux
 attribute [rsimp_optimize] Nat.Linear.Expr.toPolyFast
 
@@ -266,14 +166,14 @@ attribute [rsimp] Nat.Linear.Poly.norm_eq_sortFuse
 
 
 -- attribute [rsimp_optimize] Nat.Linear.Expr.toPoly
-attribute [rsimp] Nat.Linear.Expr.toPoly_eq_toPolyFast
+-- attribute [rsimp] Nat.Linear.Expr.toPoly_eq_toPolyFast
 
 attribute [rsimp_optimize] Nat.Linear.Expr.toNormPoly
 attribute [rsimp ←] List.reverseAux_eq
 attribute [rsimp_optimize] Nat.Linear.Poly.cancelAux
 attribute [rsimp_optimize] Nat.Linear.Poly.cancel
 
-attribute [rsimp_optimize] Nat.Linear.Var.denote.go
+-- attribute [rsimp_optimize] Nat.Linear.Var.denote.go
 attribute [rsimp_optimize] Nat.Linear.Var.denote
 -- set_option trace.tactic.rsimp_optimize true in
 attribute [rsimp_optimize] Nat.Linear.Expr.denote
@@ -300,6 +200,7 @@ theorem Nat.Linear.Expr.of_cancel_eq_opt (ctx : Context) (a b c d : Expr)
     ← Poly.cancel.eq_rsimp, Nat.Linear.Expr.toPoly'_eq_to_Poly, ← toPoly'.eq_rsimp]
   exact Expr.of_cancel_eq ctx a b c d
 
+/-
 theorem Nat.Linear.Expr.of_cancel_eq_opt_denote (ctx : Context) (a b c d : Expr)
   (h : Poly.cancel.rsimp (Expr.toNormPoly.rsimp a) (Expr.toNormPoly.rsimp b) =
     (Expr.toPolyFast.rsimp c, Expr.toPolyFast.rsimp d)) :
@@ -307,14 +208,16 @@ theorem Nat.Linear.Expr.of_cancel_eq_opt_denote (ctx : Context) (a b c d : Expr)
   (Nat.Linear.Expr.denote.rsimp ctx c = Nat.Linear.Expr.denote.rsimp ctx d) := by
   revert h
   simp only [← Expr.toNormPoly.eq_rsimp, ← Expr.toPolyFast.eq_rsimp,
-    ← Poly.cancel.eq_rsimp, ← Nat.Linear.Expr.toPoly_eq_toPolyFast,
+    ← Poly.cancel.eq_rsimp,
+    -- ← Nat.Linear.Expr.toPoly_eq_toPolyFast,
     ← Nat.Linear.Expr.denote.eq_rsimp
     ]
   exact Expr.of_cancel_eq ctx a b c d
+-/
 
 /-- warning: declaration uses 'sorry' -/
 #guard_msgs in
-theorem Nat.Linear.Expr.of_cancel_eq_opt_denote' (ctx : Data.RArray Nat) (a b c d : Expr)
+theorem Nat.Linear.Expr.of_cancel_eq_opt_denote' (ctx : Lean.RArray Nat) (a b c d : Expr)
   (h : Poly.cancel.rsimp (Expr.toNormPoly.rsimp a) (Expr.toNormPoly.rsimp b) = (Expr.toPolyFast.rsimp c, Expr.toPolyFast.rsimp d)) :
   (Nat.Linear.Expr.denote' ctx a = Nat.Linear.Expr.denote' ctx b) =
   (Nat.Linear.Expr.denote' ctx c = Nat.Linear.Expr.denote' ctx d) := by
@@ -329,7 +232,7 @@ theorem Nat.Linear.Expr.of_cancel_eq_opt_denote' (ctx : Data.RArray Nat) (a b c 
 
 /-- warning: declaration uses 'sorry' -/
 #guard_msgs in
-theorem Nat.Linear.Expr.of_cancel_eq_opt_denote'_no_rfl (ctx : Data.RArray Nat) (a b c d : Expr)
+theorem Nat.Linear.Expr.of_cancel_eq_opt_denote'_no_rfl (ctx : Lean.RArray Nat) (a b c d : Expr)
   (h : True) :
   (Nat.Linear.Expr.denote' ctx a = Nat.Linear.Expr.denote' ctx b) =
   (Nat.Linear.Expr.denote' ctx c = Nat.Linear.Expr.denote' ctx d) := by
@@ -353,26 +256,26 @@ def bench (variant : Nat) : MetaM Unit :=
       let e₁' := p₁'.toExpr
       let e₂' := p₂'.toExpr
       have _value_orig := mkApp6 (.const ``Expr.of_cancel_eq [])
-        (← mkListLit (mkConst ``Nat) xs.toList)
+        (Lean.RArray.toExpr (mkConst ``Nat) id (.ofArray xs h))
         (toExpr e₁) (toExpr e₂) (toExpr e₁') (toExpr e₂')
         (← mkEqRefl (toExpr (p₁', p₂')))
       have _value_no_rfl := mkApp5 (.const ``Expr.of_cancel_eq_no_rfl [])
-        (← mkListLit (mkConst ``Nat) xs.toList)
+        (Lean.RArray.toExpr (mkConst ``Nat) id (.ofArray xs h))
         (toExpr e₁) (toExpr e₂) (toExpr e₁') (toExpr e₂')
       have _value_opt := mkApp6 (.const ``Expr.of_cancel_eq_opt [])
-        (← mkListLit (mkConst ``Nat) xs.toList)
+        (Lean.RArray.toExpr (mkConst ``Nat) id (.ofArray xs h))
         (toExpr e₁) (toExpr e₂) (toExpr e₁') (toExpr e₂')
         (← mkEqRefl (toExpr (p₁', p₂')))
-      have _value_opt_denote := mkApp6 (.const ``Expr.of_cancel_eq_opt_denote [])
-        (← mkListLit (mkConst ``Nat) xs.toList)
+      have _value_opt_denote := mkApp6 (.const ``Expr.of_cancel_eq [])
+        (Lean.RArray.toExpr (mkConst ``Nat) id (.ofArray xs h))
         (toExpr e₁) (toExpr e₂) (toExpr e₁') (toExpr e₂')
         (← mkEqRefl (toExpr (p₁', p₂')))
       have _value_opt_denote' := mkApp6 (.const ``Expr.of_cancel_eq_opt_denote' [])
-        (Data.RArray.toExpr (mkConst ``Nat) id (.ofArray xs h))
+        (Lean.RArray.toExpr (mkConst ``Nat) id (.ofArray xs h))
         (toExpr e₁) (toExpr e₂) (toExpr e₁') (toExpr e₂')
         (← mkEqRefl (toExpr (p₁', p₂')))
       have _value_opt_denote'_no_rfl := mkApp6 (.const ``Expr.of_cancel_eq_opt_denote'_no_rfl [])
-        (Data.RArray.toExpr (mkConst ``Nat) id (.ofArray xs h))
+        (Lean.RArray.toExpr (mkConst ``Nat) id (.ofArray xs h))
         (toExpr e₁) (toExpr e₂) (toExpr e₁') (toExpr e₂')
         (mkConst ``True.intro)
       let value := match variant with
@@ -383,10 +286,10 @@ def bench (variant : Nat) : MetaM Unit :=
         | 4 => _value_opt_denote'
         | _ => _value_opt_denote'_no_rfl
       let value ← mkLambdaFVars xs value
-      let exp₁ ← Linear.Nat.LinearExpr.toArith xs e₁
-      let exp₂ ← Linear.Nat.LinearExpr.toArith xs e₂
-      let exp₁' ← Linear.Nat.LinearExpr.toArith xs e₁'
-      let exp₂' ← Linear.Nat.LinearExpr.toArith xs e₂'
+      let exp₁ ← Lean.Meta.Simp.Arith.Nat.LinearExpr.toArith xs e₁
+      let exp₂ ← Lean.Meta.Simp.Arith.Nat.LinearExpr.toArith xs e₂
+      let exp₁' ← Lean.Meta.Simp.Arith.Nat.LinearExpr.toArith xs e₁'
+      let exp₂' ← Lean.Meta.Simp.Arith.Nat.LinearExpr.toArith xs e₂'
       let type ← mkEq (← mkEq exp₁ exp₂) (← mkEq exp₁' exp₂')
       let type ← mkForallFVars xs type
 
@@ -395,7 +298,8 @@ def bench (variant : Nat) : MetaM Unit :=
       let timings : List Nat ← (List.range 5).mapM fun _ =>
         withoutModifyingEnv do
           let start ← IO.monoMsNow
-          addDecl decl
+          withOptions (Elab.async.set · false) do
+            addDecl decl
           return (← IO.monoMsNow) - start
       let some best := timings.min? | unreachable!
       logInfo m!"time {variant}: {best}ms"
